{
 "cells": [
  {
   "cell_type": "markdown",
   "metadata": {},
   "source": [
    "# Derivative Formulas\n",
    "http://tutorial.math.lamar.edu/pdf/Calculus_Cheat_Sheet_All.pdf\n",
    "\n",
    "$\\newcommand{\\dv}{\\displaystyle \\frac{d}{dx}}$\n",
    "$\\newcommand{\\ds}{\\displaystyle}$\n",
    "    \n",
    "----\n",
    "\n",
    "### Limits - Definition\n",
    "#### Precise Definition\n",
    "$\\displaystyle\\lim_{x\\to\\alpha} f(x) = L$ \n",
    "if for every $\\epsilon > 0$, there is  $\\delta > 0$, such that whenever $0 < |x-\\alpha| < \\delta$ then $|f(x) - L| < \\epsilon$\n",
    "#### Working Definition\n",
    "We say $\\displaystyle\\lim_{x\\to\\alpha} f(x) = L$ \n",
    "if we can make f(x) as close to L as we want by taking x sufficiently close to $\\alpha$ (on either side of $\\alpha$) without letting x = $\\alpha$.\n",
    "#### Right Hand Limit Definition\n",
    "$\\displaystyle\\lim_{x\\to\\alpha^+} f(x) = L$, \n",
    "same definition as above, abd x>$\\alpha$\n",
    "#### Left Hand Limit Definition\n",
    "$\\displaystyle\\lim_{x\\to\\alpha^+} f(x) = L$, \n",
    "same definition as above, and x<$\\alpha$\n",
    "\n"
   ]
  },
  {
   "cell_type": "markdown",
   "metadata": {},
   "source": [
    "\n",
    "----\n",
    "### Basic Derivatives\n",
    "$\\ds \\begin{equation} \\label{eq1}\n",
    "\\begin{split}\n",
    "(c f)^\\prime & = c f^{\\prime}(x), c\\in\\mathbb{R} \\ \\\\\n",
    "\\\\\n",
    "(f \\pm g)^\\prime & = f^{\\prime}(x) \\pm g^{\\prime}(x) \\\\\n",
    "\\\\\n",
    "(f g)^\\prime & = f^{\\prime}g + fg^{\\prime} \\\\\n",
    "\\\\\n",
    "\\left(\\frac{f}{g}\\right)^\\prime & = \\frac{f^{\\prime}g - fg^{\\prime}}{g^2} \\\\\n",
    "\\\\\n",
    "\\dv\\Big( f\\big(g(x)\\big)\\Big) & = f^{\\prime}\\big(g(x)\\big)\\;g^{\\prime}(x) \\\\\n",
    "\\end{split}\n",
    "\\end{equation}$\n",
    "\n",
    "----\n",
    "\n",
    "\n",
    "\n",
    "| Formula Example Formula Example | Derivative Formula Derivative Formula |\n",
    "| -- | -- |\n",
    "| $\\dv f( c ) = 0 $ | $\\dv f( sin\\;x ) = \\ds cos\\;x $ |\n",
    "| $\\dv f( x ) = 1 $ | $\\dv f( cos\\;x ) = \\ds -sin\\;x $ |\n",
    "| $\\dv f( x^a ) = ax^{a-1} $ | $\\dv f( tan\\;x ) = \\ds sec^2\\;x $ |\n",
    "| $\\dv f( a^x ) = a^x\\ln(a) $ | $\\dv f( sec\\;x ) = \\ds sec\\;x\\;tan\\;x $ |\n",
    "| $\\dv f( e^x ) = e^x $ | $\\dv f( csc\\;x ) = \\ds -csc\\;x\\;cot\\;x $ |\n",
    "| $\\dv f( ln(x) ) = \\frac{1}{x}, x > 0 $ | $\\dv f( cot\\;x ) = \\ds -csc^2\\;x $ |\n",
    "| $\\dv f( ln|x| ) = \\frac{1}{x}, x \\ne 0 $ |\n",
    "| $\\dv f( log_a(x) ) = \\frac{1}{x ln(a)}, x > 0 $ |\n",
    "\n",
    "### Notes\n",
    "| Formula Rule | Formula Example Formula Example | Related Derivative Formula | Where Condition |\n",
    "| -- | -- | -- | -- |\n",
    "| | $\\ds f(x) = ax^b + c$ | $\\ds \\frac{d}{dx}f(x) = abx^{b-1} dx $ |\n",
    "| | $\\ds f(x) = a_1x^b_1 + a_2x^b_2 + c$ | $\\displaystyle \\frac{d}{dx}f(x) = a_1b_1x^{b_1-1} + a_2b_2x^{b_2-1} dx $ |\n",
    "| | $\\ds f(x) = e^x + c $ | $\\ds \\frac{d}{dx}f(x) = e ^x dx $ |\n",
    "| | $\\ds f(x) = ln(x) + c $ | $\\ds \\frac{d}{dx}f(x) = x^{-1} dx $ |\n",
    "| | $\\ds \\big(\\alpha\\;f(x)\\big)^{\\prime} = \\alpha\\;f^{\\prime}(x) $ | $\\dv \\big(\\alpha\\;f(x)\\big) = \\alpha\\;\\dv f(x)$ | $\\alpha\\in\\mathbb{R}$ |\n",
    "| Sum Rule | $\\ds (f \\pm g)^{\\prime} $ | $\\ds f^{\\prime}(x) \\pm g^{\\prime}(x)$ | |\n",
    "| | $\\dv \\Big( \\sum_{i=1}^{n} f_i(x) \\Big)$ | $\\ds \\sum_{i=1}^{n} \\dv f_i(x) $ | |\n"
   ]
  },
  {
   "cell_type": "markdown",
   "metadata": {},
   "source": [
    "----\n",
    "### Basic Integrals\n",
    "$\\newcommand{\\dv}{\\displaystyle \\frac{d}{dx}}$\n",
    "$\\newcommand{\\ds}{\\displaystyle}$\n",
    "\n",
    "$\\ds \\begin{equation} \\label{eq1}\n",
    "\\begin{split}\n",
    "\\text{Integratation by parts} \\\\\n",
    "\\int u.\\frac{d(v)}{dx} &= uv - \\int v.\\frac{d(u)}{dx} dx \\\\\n",
    "\\end{split}\n",
    "\\end{equation}$\n",
    "\n",
    "----"
   ]
  },
  {
   "cell_type": "markdown",
   "metadata": {},
   "source": [
    "### Integration by Parts\n",
    "#### Derivation\n",
    "$\\newcommand{\\dv}{\\displaystyle \\frac{d}{dx}}$\n",
    "$\\newcommand{\\ds}{\\displaystyle}$\n",
    "$\\ds \\begin{equation} \\label{eq1}\n",
    "\\begin{split}\n",
    "y & = u v \\\\\n",
    "\\frac{dy}{dx} & = \\frac{d(uv)}{dx} \\\\\n",
    "\\frac{d(uv)}{dx} & = u.\\frac{d(v)}{dx} + v.\\frac{d(u)}{dx} \\\\\n",
    "\\text{rearrange...} \\\\\n",
    "u.\\frac{d(v)}{dx} & = \\frac{d(uv)}{dx} - v.\\frac{d(u)}{dx} \\\\\n",
    "\\text{integrate both sides} \\\\\n",
    "\\int u.\\frac{dv}{dx} dx & = \\int \\Big( \\frac{d(uv)}{dx} - v.\\frac{du}{dx} \\Big) dx \\\\\n",
    "\\int u.\\frac{dv}{dx} dx & = \\int \\frac{d(uv)}{dx} dx - \\int v.\\frac{du}{dx} dx \\\\\n",
    "\\text{formula:} \\\\\n",
    "\\int u.\\frac{dv}{dx} dx & = u.v - \\int v.\\frac{du}{dx} dx \\\\\n",
    "\\end{split}\n",
    "\\end{equation}$\n",
    "\n",
    "---"
   ]
  },
  {
   "cell_type": "markdown",
   "metadata": {},
   "source": [
    "### Quadratic Formula\n",
    "#### Derivation\n",
    "$\\newcommand{\\dv}{\\displaystyle \\frac{d}{dx}}$\n",
    "$\\newcommand{\\ds}{\\displaystyle}$\n",
    "(from https://www.mathsisfun.com/algebra/completing-square.html)\n",
    "\n",
    "\n",
    "$\\ds \\begin{equation} \\label{quadratic}\n",
    "\\begin{split}\n",
    "ax^2 + bx + c & = 0 \\\\\n",
    "x^2 + \\frac{b}{a}x + \\frac{c}{a} & = 0  \\\\\n",
    "x^2 + \\frac{b}{a}x & = - \\frac{c}{a}  \\\\\n",
    "\\text{complete the square} \\\\\n",
    "\\Big(x + \\frac{b}{2a}\\Big)^2 - \\Big(\\frac{b}{2a}\\Big)^2 & = - \\frac{c}{a}  \\\\\n",
    "\\text{complete the square} \\\\\n",
    "\\Big(x + \\frac{b}{2a}\\Big)^2 & = - \\frac{c}{a} + \\Big(\\frac{b}{2a}\\Big)^2 \\\\\n",
    "\\Big(x + \\frac{b}{2a}\\Big)^2 & = - \\frac{c}{a} + \\frac{b^2}{(2a)^2} \\\\\n",
    "\\Big(x + \\frac{b}{2a}\\Big)^2 & = - \\frac{4ac}{4a^2} + \\frac{b^2}{(2a)^2} \\\\\n",
    "\\Big(x + \\frac{b}{2a}\\Big)^2 & = \\frac{b^2 - 4ac}{(2a)^2} \\\\\n",
    "x + \\frac{b}{2a} & = \\pm \\sqrt{ \\frac{b^2 - 4ac}{(2a)^2} } \\\\\n",
    "x & = \\frac{\\pm \\sqrt{ b^2 - 4ac}}{2a} - \\frac{b}{2a}\\\\\n",
    "x & = \\frac{-b \\pm \\sqrt{ b^2 - 4ac}}{2a}\\\\\n",
    "\\end{split}\n",
    "\\end{equation}$\n"
   ]
  },
  {
   "cell_type": "code",
   "execution_count": null,
   "metadata": {},
   "outputs": [],
   "source": []
  }
 ],
 "metadata": {
  "kernelspec": {
   "display_name": "Python 3",
   "language": "python",
   "name": "python3"
  },
  "language_info": {
   "codemirror_mode": {
    "name": "ipython",
    "version": 3
   },
   "file_extension": ".py",
   "mimetype": "text/x-python",
   "name": "python",
   "nbconvert_exporter": "python",
   "pygments_lexer": "ipython3",
   "version": "3.6.5"
  }
 },
 "nbformat": 4,
 "nbformat_minor": 2
}
